

hadi jo

~~Previous assignments from class~~

UNIT-3 Fourier



nm

Time to frequency
It's useful in solving boundary value problems.
like heat, wave etc

Complex exponential form

If $f(x)$ is periodic func of period $2L$ defined in $-L \leq x \leq L$ & satisfies Dirichlet's condition ($f(x)$ must have finite max & min, max finite no. of discontinuities & $f(x)$)

Then $f(x)$ is represented as

$$\left\{ f(x) = \frac{a_0}{2} + \sum_{n=1}^{\infty} \left(a_n \cos \frac{n\pi x}{L} + b_n \sin \frac{n\pi x}{L} \right) \right\} \quad \text{***}$$

$$\text{Where } a_0 = \frac{1}{L} \int_{-L}^L f(u) du$$

$$a_n = \frac{1}{L} \int_{-L}^L f(u) \cos \frac{n\pi u}{L} du$$

$$b_n = \frac{1}{L} \int_{-L}^L f(u) \sin \frac{n\pi u}{L} du$$

$$\text{using } \therefore \cos \theta = \frac{e^{i\theta} + e^{-i\theta}}{2}, \sin \theta = \frac{e^{i\theta} - e^{-i\theta}}{2i} = \frac{-i}{2} (e^{i\theta} - e^{-i\theta})$$

$\theta = \frac{n\pi x}{L}$

$$f(x) = \frac{a_0}{2} + \sum_{n=1}^{\infty} + \sum_{n=1}^{\infty} \left[a_n \left(\frac{e^{\frac{i n \pi x}{L}} + e^{-\frac{i n \pi x}{L}}}{2} \right) + b_n \left(\frac{e^{\frac{i n \pi x}{L}} - e^{-\frac{i n \pi x}{L}}}{2} \right) \right]$$

$$f(x) = \frac{a_0}{2} + \sum_{n=1}^{\infty} \left[\left(\frac{a_n - i b_n}{2} \right) e^{\frac{i n \pi x}{L}} + \left(\frac{a_n + i b_n}{2} \right) e^{-\frac{i n \pi x}{L}} \right]$$

$$f(x) = c_0 + \sum_{n=1}^{\infty} \left[c_n e^{\frac{i n \pi x}{L}} + c_n e^{-\frac{i n \pi x}{L}} \right]$$

$$\left\{ f(x) = \sum_{n=-\infty}^{\infty} c_n e^{\frac{i n \pi x}{L}} \right\} \quad \text{---D---} \quad \text{***}$$

When $c_n = \frac{a_n - ib_n}{2}$

$$= \frac{1}{2} \left[\frac{1}{L} \int_{-L}^L f(u) \cos \frac{n\pi u}{L} du - i \frac{1}{L} \int_{-L}^L f(u) \sin \frac{n\pi u}{L} du \right]$$

$$= \frac{1}{2L} \left[\int_{-L}^L f(u) \left(\cos \frac{n\pi u}{L} - i \sin \frac{n\pi u}{L} \right) du \right]$$

$$\left\{ c_n = \frac{1}{2L} \left[\int_{-L}^L f(u) e^{-i \frac{n\pi u}{L}} du \right] \right\} \quad **$$

$$c_{-n} = \frac{1}{2L} \left[\int_{-L}^L f(u) e^{i \frac{n\pi u}{L}} du \right] \quad (2)$$

$\therefore$ complex form of Fourier is obtained by (1) & (2)

* Fourier Integral

We will now consider the limiting form of Fourier series for periodic func of period $2L$ where $L \rightarrow \infty$

We know

$$f(x) = \sum_{n=-\infty}^{\infty} c_n e^{i \frac{n\pi x}{L}} \quad (1)$$

where

$$c_n = \frac{1}{2L} \left[\int_{-L}^L f(u) e^{-i \frac{n\pi u}{L}} du \right] \quad (2)$$

Put (2) in (1)

$$f(x) = \sum_{n=-\infty}^{\infty} \left[\frac{1}{2L} \left(\int_{-L}^L f(u) e^{-\frac{i n \pi u}{L}} du \right) e^{\frac{i n \pi x}{L}} \right]$$

$$= \sum_{n=-\infty}^{\infty} \frac{1}{2L} \left[\int_{-L}^L f(u) e^{-\frac{i n \pi (u-x)}{L}} du \right]$$

$$\text{Let } \left[\frac{x}{L} = \frac{n\pi}{L} \right] \quad \Delta \lambda = \frac{(n+1)\pi}{L} - \frac{n\pi}{L}$$

$$= \frac{n\pi}{L} + \frac{\pi}{L} - \frac{n\pi}{L}$$

$$\Delta \lambda = \frac{\pi}{L}$$

$$= \sum_{n=-\infty}^{\infty} \frac{1}{2\pi} \left(\frac{\pi}{L} \right) \left[\int_{-L}^L f(u) e^{-\frac{i n \pi (u-x)}{L}} du \right]$$

$$f(x) = \sum_{n=-\infty}^{\infty} \frac{1}{2\pi} \left[\int_{-L}^L f(u) e^{-i \lambda (u-x)} du \right] \Delta \lambda$$

$$= \lim_{L \rightarrow \infty} \sum_{n=-\infty}^{\infty} \frac{1}{2\pi} \left[\int_{-L}^L f(u) e^{-i \lambda (u-x)} du \right] \Delta \lambda$$

$$\lim_{\Delta \lambda \rightarrow 0} \sum_{n=-\infty}^{\infty} \frac{1}{2\pi} \left[\int_{-L}^L f(u) e^{-i \lambda (u-x)} du \right] \Delta \lambda$$

$$\lim_{\Delta \lambda \rightarrow 0} \sum_{n=-\infty}^{\infty} f(x) = \frac{1}{2\pi} \int_{-\infty}^{\infty} \int_{-\infty}^{\infty} f(u) e^{-i \lambda (u-x)} du d\lambda$$

FOURIER INTEGRAL



Equivalent forms of fourier integral

Various forms

We know

$$f(x) = \frac{1}{2\pi} \int_{-\infty}^{\infty} \int_{-\infty}^{\infty} f(u) e^{-ix(u-x)} du dx$$

$$= \frac{1}{2\pi} \int_{-\infty}^{\infty} \int_{-\infty}^{\infty} f(u) [\cos x(u-x) - i \sin x(u-x)] du dx$$

$$= \frac{1}{2\pi} \left[\int_{-\infty}^{\infty} \int_{-\infty}^{\infty} f(u) \cos x(u-x) du dx - \right.$$

$$\left. i \int_{-\infty}^{\infty} \int_{-\infty}^{\infty} f(u) \sin x(u-x) du dx \right]$$

Since $\sin x(u-x)$ is odd func of x

$$\therefore \int_{-\infty}^{\infty} \sin x(u-x) dx = 0$$

$$f(x) = \frac{1}{2\pi} \int_{-\infty}^{\infty} \int_{-\infty}^{\infty} f(u) \cos x(u-x) du dx$$

$$= \cos x(u-x)$$

We know

$$\int_{-\infty}^{\infty} \cos x(u-x) dx \rightarrow 2 \int_0^{\infty} \cos x(u-x) dx$$

$$f(x) = \frac{1}{\pi} \int_0^{\infty} \int_{-\infty}^{\infty} f(u) \cos x(u-x) du dx$$

$$f(x) = \frac{1}{\pi} \int_{\lambda=0}^{\infty} \int_{u=-\infty}^{\infty} f(u) [\cos \lambda u \cos \lambda x + \sin \lambda u \sin \lambda x] du d\lambda$$

This is equivalent form of fourier integral — (4)

Case 1: If $f(x)$ is an even func. then

① $f(u) \sin \lambda u = \text{odd func.} \rightarrow \int_{-\infty}^{\infty} f(u) \sin \lambda u = 0$

$$\therefore f(x) = \frac{1}{\pi} \int_{\lambda=0}^{\infty} \int_{u=-\infty}^{\infty} f(u) \cos \lambda u \cos \lambda x du d\lambda$$

② Since it is even func.,

$\therefore$ we have

$$\left\{ f(x) = \frac{2}{\pi} \int_{\lambda=0}^{\infty} \int_{u=-\infty}^{\infty} f(u) \cos \lambda u \cos \lambda x du d\lambda \right\} ** \quad \text{--- (5)}$$

(5) is fourier cosine integral of $f(x)$

Case 2: If $f(x)$ is an odd func. then

~~Example~~

$$f(u) \cos \lambda u \rightarrow \text{odd}$$

$$\int_{-\infty}^{\infty} f(u) \cos \lambda u = 0$$

$$\therefore f(x) = \frac{1}{\pi} \int_{\lambda=0}^{\infty} \int_{u=-\infty}^{\infty} f(u) \sin \lambda u \sin \lambda x du d\lambda$$

$$\int_{-\infty}^{\infty} f(u) \sin \lambda u = \text{even} = 2 \int_0^{\infty} f(u) \sin \lambda u du$$

$$\left\{ f(x) = \frac{2}{\pi} \int_{\lambda=0}^{\infty} \int_{u=0}^{\infty} f(u) \sin \lambda u \sin \lambda x du d\lambda \right\} ** \quad \text{--- (6)}$$

(6) is fourier sine integral representation

Fourier sine & cosine transform

Eg 5 can be written as

$$f(x) = \frac{2}{\pi} \int_0^{\infty} \left[\int_0^{\infty} f(u) \cos xu \, du \right] \cos x \, dx$$

$$F_c(x) = \int_0^{\infty} f(u) \cos xu \, du$$

Inverse Fourier cosine transform

$$F_c(x) = f(x) = \frac{2}{\pi} \int_0^{\infty} F_c(x) \cos xu \, dx$$

$$-\infty < x < \infty$$

$$f(x) = \frac{2}{\pi} \int_0^{\infty} \left[\int_0^{\infty} f(u) \sin xu \, du \right] \sin x \, dx$$

Fourier
sine transform

$$F_s(x) = \int_0^{\infty} f(u) \sin xu \, du$$

$$F_s(x) = f(x) = \frac{2}{\pi} \int_0^{\infty} F_s(x) \sin xu \, dx$$

* If $f(x)$ is even func. defined in $0 < x < \infty$ then we use Fourier cosine T. eg 7 or 8

If $f(x)$ is an odd func. defined in $0 < x < \infty$ then we use Fourier sine T. ie eg 9 & 10

If $f(x)$ is neither E or O then we use generalised Fourier transform ie (11) or (12)

Name of transformation

Interval

Transformation

Inverse

1. Fourier

$$-\infty < x < \infty$$

$$f(x) = \int_{-\infty}^{\infty} f(u) e^{-i\pi u} du$$

$$f(u) = \frac{1}{2\pi} \int_{-\infty}^{\infty} f(x) e^{i\pi x} dx$$

2. Fourier cosine (even)

$$-\infty < x < \infty$$

$$F_c(x) = \int_0^{\infty} f(u) \cos \pi u du$$

$$f(u) = 2 \int_0^{\infty} F_c(x) \cos \pi x dx$$

3. Fourier sine (odd)

$$-\infty < x < \infty$$

$$F_s(x) = \int_0^{\infty} f(u) \sin \pi u du$$

$$f(u) = \frac{2}{\pi} \int_0^{\infty} F_s(x) \sin \pi x dx$$

4. Fourier cosine

$$0 < x < \infty$$

$$F_c(x) = \int_0^{\infty} f(u) \cos \pi u du$$

$$f(u) = \frac{2}{\pi} \int_0^{\infty} F_c(x) \cos \pi x dx$$

5. Fourier sine

$$0 < x < \infty$$

$$F_s(x) = \int_0^{\infty} f(u) \sin \pi u du$$

$$f(u) = \frac{2}{\pi} \int_0^{\infty} F_s(x) \sin \pi x dx$$

Pre-requisites

$$1) \int_0^{\infty} e^{ax} \cos bx dx = \frac{e^{ax}}{a^2 + b^2} (a \cos bx + b \sin bx)$$

$$2) \int_0^{\infty} e^{ax} \sin bx dx = \frac{e^{ax}}{a^2 + b^2} (a \sin bx - b \cos bx)$$

$$3) \int_0^{\infty} e^{-ax} \cos bx dx = \frac{a}{a^2 + b^2}$$

$$4) \int_0^{\infty} e^{-ax} \sin bx dx = \frac{b}{a^2 + b^2}$$

$$5) \int_0^{2\pi} \cos(mx) \cos(nx) dx = 0 \text{ where } m \neq n$$

$$= \pi, m = n$$

$$6) e^{ix} = \cos x + i \sin x$$

$$e^{-ix} = \cos x - i \sin x$$

$$8. \int_0^{\infty} \frac{\sin ax}{x} dx = \frac{\pi}{2}, a > 0$$

$$= -\frac{\pi}{2}, a < 0$$

$$9. \sin x = \frac{e^{ix} - e^{-ix}}{2i}$$

$$10. \cos x = \frac{e^{ix} + e^{-ix}}{2}$$

Type 1: Fourier Integral Rep.

Q1. Find the Fourier transform & also give the Fourier integral representation.

$$1) f(x) = 1 \quad 0 \leq x \leq 1$$

$$= 0 \quad x < 0, x > 1$$

i. The F.I.T is given by

$$f(x) = \int_{-\infty}^{\infty} f(u) e^{-ixu} du$$

$$= \int_0^1 (1) e^{-ixu} du$$

$$= \left[\frac{-e^{-ixu}}{ix} \right]_0^1$$

$$= -\frac{1}{ix} [e^{-ix} - e^0]$$

$$f(x) = \frac{i}{x} [e^{-ix} - 1]$$

$$ii. \text{F.I.R : } f(x) = \frac{1}{2\pi} \int_{-\infty}^{\infty} \left[\int_{-\infty}^{\infty} f(u) e^{-ixu} du \right] e^{ixu} dx$$

$$= \frac{1}{2\pi} \int_{-\infty}^{\infty} f(u) e^{ixu} dx$$

$$\therefore f(x) = \frac{1}{2\pi} \int_{-\infty}^{\infty} \frac{i(e^{i\lambda} - 1)e^{i\lambda x}}{\lambda} d\lambda$$

2] Find F.I.R.

$$f(x) = 1, |x| \leq 1$$

$$= 0, |x| > 1$$

and evaluate $\int \frac{\sin \lambda \cos \lambda x}{\lambda} d\lambda = \int \frac{\sin \lambda}{\lambda} d\lambda$

$\therefore F(x)$ is an even func. $\therefore$ we use $F_c(x)$

i $F_c(x) = \int_0^{\infty} f(u) \cos \lambda x du$

$$= \int_0^1 (1) \cos \lambda x du$$

$$= \left[\frac{\sin \lambda x}{\lambda} \right]_0^1$$

$$F_c(x) = \frac{\sin x}{x}$$

ii The fourier cosine integral rep is given by

$$f(x) = \frac{2}{\pi} \int_0^{\infty} \left[\int_0^{\infty} f(u) \cos \lambda u du \right] \cos \lambda x d\lambda$$

$$f(x) = \frac{2}{\pi} \int_0^{\infty} \frac{\sin \lambda}{\lambda} \cos \lambda x d\lambda$$

$$(\#) f(x) \frac{\pi}{2} = \int_0^{\infty} \frac{\sin \lambda \cos \lambda x}{\lambda} d\lambda$$

$$(1) \frac{\pi}{2} = \int_0^{\infty} \frac{\sin \lambda \cos \lambda x}{\lambda} d\lambda, |x| \leq 1$$

$$\int_0^{\infty} \frac{\sin \lambda \cos \lambda x}{\lambda} d\lambda = 0, |x| > 1$$

iii We know that;

$$\int_{-\infty}^{\infty} \frac{\sin \lambda \cos \lambda x}{\lambda} d\lambda = f(x) \frac{\pi}{2}$$

Put $x = 0$

$$\int_{-\infty}^{\infty} \frac{\sin \lambda}{\lambda} d\lambda = f(0) \frac{\pi}{2}$$

$$\therefore \int_{-\infty}^{\infty} \frac{\sin \lambda}{\lambda} d\lambda = \frac{\pi}{2}$$

By considering fourier sine & cosine transformation of:

$$f(x) = e^{-mx} \quad (m > 0)$$

1) Prove that $\int_{-\infty}^{\infty} \frac{\lambda \sin \lambda x}{\lambda^2 + m^2} d\lambda = \pi e^{-mx}$

2) Prove that $\int_{-\infty}^{\infty} \frac{\cos \lambda x}{\lambda^2 + m^2} d\lambda = \frac{\pi}{2m} e^{-mx}$

fourier sine trans is given by

$$F_s(\lambda) = \int_{-\infty}^{\infty} f(x) \sin \lambda x dx$$

$$= \int_{-\infty}^{\infty} e^{-mx} \sin \lambda x dx$$

$$F_s(\lambda) = \frac{\lambda}{\lambda^2 + m^2}$$

By fourier sine integral

$$f(x) = \frac{2}{\pi} \int_0^{\infty} F_s(\lambda) \sin \lambda x d\lambda$$

$$e^{-mx} = \frac{2}{\pi} \int_0^{\infty} \frac{\lambda \sin \lambda x}{\lambda^2 + m^2} d\lambda$$

$$\left| \int_{-\infty}^{\infty} \frac{2}{\lambda^2 + m^2} \sin \lambda x \, d\lambda = \frac{\pi e^{-m|x|}}{2} \right|$$

fourier cosine trans is given by

$$F_c(\lambda) = \int_0^{\infty} f(u) \cos \lambda u \, du$$

$$= \int_0^{\infty} e^{-mu} \cos \lambda u \, du$$

$$F_c(\lambda) = \frac{m}{\lambda^2 + m^2}$$

By fourier cosine integral

$$f(x) = \frac{2}{\pi} \int_0^{\infty} F_c(\lambda) \cos \lambda x \, d\lambda$$

$$e^{-mx} = \frac{2m}{\pi} \int_0^{\infty} \frac{1}{\lambda^2 + m^2} \cos \lambda x \, d\lambda$$

$$\left| \frac{\pi e^{-mx}}{2m} = \int_0^{\infty} \frac{1}{\lambda^2 + m^2} \cos \lambda x \, d\lambda \right|$$

4. Show that the fourier transform of $f(x) = e^{-|x|}$ is $\frac{2}{1+\lambda^2}$

* To check if the func. is even or odd Put $x = -x$
if func is 0 then odd.

Put $x = -1$

$$f(-x) = e^{-|-x|} = e^{-|x|} = \text{even}$$

Hence we use fourier cosine transform

$$F_c(\lambda) = \int_0^{\infty} f(u) \cos \lambda u \, du$$

$$= \int_0^{\infty} e^{-u} \cos \lambda u \, du$$

Q5. Find the fourier sine transform of

$$f(x) = \begin{cases} x, & 0 \leq x \leq a \\ 0, & x > a \end{cases}$$

By fourier sine transform

$$F_s(\lambda) = \int_0^a f(x) \sin \lambda x dx$$

$$= \int_0^a x \sin \lambda x dx + \int_a^\infty 0 \sin \lambda x dx$$

$$= \left[x \left(-\frac{\cos \lambda x}{\lambda} \right) - \left(\frac{\sin \lambda x}{\lambda^2} \right) \right]_0^a$$

$$F_s(\lambda) = \frac{\sin \lambda a}{\lambda^2} - \frac{a \cos \lambda a}{\lambda}$$

$$f(u) = \begin{cases} 0 & u < 0 \\ e^{-u} & u > 0 \\ \frac{1}{2} & u = 0 \end{cases}$$

By using Fourier trans

$$F(\lambda) = \int_{-\infty}^{\infty} f(u) e^{-i\lambda u} du$$

$$= \int_0^{\infty} e^{-u} e^{-i\lambda u} du$$

$$= \int_0^{\infty} e^{-u(1+i\lambda)} du$$

$$= \left[\frac{e^{-u(1+i\lambda)}}{-(1+i\lambda)} \right]_0^{\infty}$$

$$= \frac{1}{1+i\lambda}$$

$$= \frac{1-i\lambda}{(1+i\lambda)(1-i\lambda)}$$

$$= \frac{1-i\lambda}{1+\lambda^2}$$

Now Fourier Integral

$$f(u) = \frac{1}{2\pi} \int_{-\infty}^{\infty} F(\lambda) e^{i\lambda u} d\lambda$$

$$= \frac{1}{2\pi} \int_{-\infty}^{\infty} \frac{1-i\lambda}{1+\lambda^2} (\cos \lambda u + i \sin \lambda u) d\lambda$$

$$= \frac{1}{2\pi} \int_{-\infty}^{\infty} \frac{1}{1+\lambda^2} (\cos \lambda u + i \sin \lambda u - i \lambda \cos \lambda u + \lambda \sin \lambda u) d\lambda$$

$$= \frac{1}{2\pi} \int_{-\infty}^{\infty} \frac{1}{1+\lambda^2} (\cos \lambda u + \lambda \sin \lambda u) d\lambda - i \frac{1}{2\pi} \int_{-\infty}^{\infty} \frac{(\sin \lambda u - \lambda \cos \lambda u)}{1+\lambda^2} d\lambda$$

Even

$f(u)$

Odd

$g(u) = 0$

$$= \frac{2}{2\pi} \int_0^{\infty} \frac{1}{1+\lambda^2} (\cos \lambda x + \lambda \sin \lambda x) d\lambda + 0$$

$$f(x) = \frac{1}{\pi} \int_0^{\infty} \frac{1}{1+\lambda^2} (\cos \lambda x + \lambda \sin \lambda x) d\lambda$$

2. Find fourier integral cosine function

$$f(x) = \begin{cases} x^2, & 0 < x < a \\ 0, & x > a \end{cases}$$

Fourier cosine transform

$$f_c(\lambda) = \int_0^{\infty} f(x) \cos \lambda x dx$$

$$= \int_0^a x^2 \cos \lambda x dx$$

$$\left[x^2 \left(\frac{\sin \lambda x}{\lambda} \right) - (2x) \left(\frac{-\cos \lambda x}{\lambda^2} \right) + 2 \left(\frac{-\sin \lambda x}{\lambda^3} \right) \right]_0^a$$

$$f_c(\lambda) = \frac{a^2 \sin \lambda a}{\lambda} + \frac{2a \cos \lambda a}{\lambda^2} - \frac{2 \sin \lambda a}{\lambda^3}$$

Now, F.I.R,

$$f(x) = \frac{2}{\pi} \int_0^{\infty} f_c(\lambda) \cos \lambda x d\lambda$$

$$f(x) = \frac{2}{\pi} \int_0^{\infty} \left(\frac{a^2 \sin \lambda a}{\lambda} + \frac{2a \cos \lambda a}{\lambda^2} - \frac{2 \sin \lambda a}{\lambda^3} \right) \cos \lambda x d\lambda$$

$\lambda u + u$
 ~~$\lambda u + u$~~
 λu

Quick Work

Page No.:

Date:

M T W T F S S

Q. using fourier integral representation show that
 $\int_0^{\infty} \frac{\lambda^3}{\lambda^4 + 4} \sin \lambda x \, d\lambda = \frac{\pi}{2} e^{-x} \cos x, x > 0$

By using fourier sin transf,
 $F_s(\lambda) = \int_0^{\infty} f(u) \sin \lambda u \, du$

$$= \frac{\pi}{2} \int_0^{\infty} e^{-u} \cos u \sin \lambda u \, du$$

$a=1, b=\lambda$

$$\frac{\pi}{4} \int_0^{\infty} e^{-u} [\sin(\lambda+1)u + \sin(\lambda-1)u] \, du$$

$$= \frac{\pi}{4} \left[\int_0^{\infty} e^{-u} \sin(\lambda+1)u \, du + \int_0^{\infty} e^{-u} \sin(\lambda-1)u \, du \right]$$

$a=1, b=\lambda+1 \quad a=1, b=\lambda-1$

$$= \frac{\pi}{4} \left[\frac{\lambda+1 - 1}{(\lambda+1)^2 + 1} + \frac{\lambda-1 - 1}{(\lambda-1)^2 + 1} \right]$$

$$= \frac{\pi}{4} \left[\frac{\lambda+1}{\lambda^2 + 2\lambda + 2} + \frac{\lambda-1}{\lambda^2 - 2\lambda + 2} \right]$$

$$\frac{\pi}{4} \left[\frac{2\lambda^3}{\lambda^4 + 4} \right]$$

$$F_s(\lambda) = \frac{\pi}{2} \left(\frac{\lambda^3}{\lambda^4 + 4} \right) \quad \text{--- (1)}$$

By using fourier integral sine rep.
 FSIR

$$f(x) = \frac{2}{\pi} \int_0^{\infty} F_s(\lambda) \sin \lambda x \, d\lambda$$

$$= \frac{2}{\pi} \int_0^{\infty} \frac{\pi}{2} \left(\frac{\lambda^3}{\lambda^4 + 4} \right) \sin \lambda x \, d\lambda$$

$$\frac{\pi}{2} e^{-x} \cos x = \int_0^{\infty} \frac{\lambda^3}{\lambda^4 + 4} \sin \lambda x \, d\lambda$$

Put value of four trans in inverse and don't solve further.

Type-2 Problems on Fourier transform

Q1. Find Fourier sine & cosine transform of following function

$$1) f(u) = \begin{cases} u & 0 \leq u \leq 1 \\ 2-u & 1 \leq u \leq 2 \\ 0 & u > 2 \end{cases}$$

~~f(x)~~

$$F_c(\lambda) = \int_0^{\infty} f(u) \cos \lambda u \, du$$

$$= \int_0^1 u \cos \lambda u \, du + \int_1^2 (2-u) \cos \lambda u \, du + 0$$

$$= \left[u \left(\frac{\sin \lambda u}{\lambda} \right) - (1) \left(\frac{-\cos \lambda u}{\lambda^2} \right) \right]_0^1 + \left[(2-u) \left(\frac{\sin \lambda u}{\lambda} \right) - (-1) \left(\frac{-\cos \lambda u}{\lambda^2} \right) \right]_1^2$$

$$\left[\frac{\sin \lambda}{\lambda} + \frac{\cos \lambda}{\lambda^2} - \frac{1}{\lambda^2} \right] + \left[\frac{-\cos 2\lambda}{\lambda^2} - \frac{\sin \lambda}{\lambda} + \frac{\cos \lambda}{\lambda^2} \right]$$

$$F_c(\lambda) = \frac{2 \cos \lambda}{\lambda^2} - \frac{1}{\lambda^2} - \frac{\cos 2\lambda}{\lambda^2}$$

Similarly:

$$F_s(\lambda) = \int_0^{\infty} f(u) \sin \lambda u \, du$$

$$= \int_0^1 u \sin \lambda u \, du + \int_1^2 (2-u) \sin \lambda u \, du + 0$$

$$\left[u \left(\frac{-\cos \lambda u}{\lambda} \right) + (1) \left(\frac{-\sin \lambda u}{\lambda^2} \right) \right]_0^1 + \left[(2-u) \left(\frac{-\cos \lambda u}{\lambda} \right) - (-1) \left(\frac{-\sin \lambda u}{\lambda^2} \right) \right]_1^2$$

psw



Quick Work

Page No.:

Date:

M T W T F S S

$$\left(\frac{-\cos \lambda - \frac{\sin \lambda}{\lambda^2}}{\lambda} \right) + \left(\frac{-\sin 2\lambda}{\lambda^2} \right) - \left(\frac{-\cos \lambda - \frac{\sin \lambda}{\lambda^2}}{\lambda} \right)$$

$$\left[\frac{-\cos \lambda - \frac{\sin \lambda}{\lambda^2}}{\lambda} \right] + \left[\frac{-\sin 2\lambda}{\lambda^2} + \frac{\cos \lambda + \frac{\sin \lambda}{\lambda^2}}{\lambda} \right]$$

$$\frac{-\cos \lambda - \frac{\sin \lambda}{\lambda^2}}{\lambda} - \frac{\sin 2\lambda}{\lambda^2} + \frac{\cos \lambda + \frac{\sin \lambda}{\lambda^2}}{\lambda}$$

$$\frac{-\sin 2\lambda}{\lambda^2}$$

$$2) f(x) = \begin{cases} \cos x, & 0 < x < a \\ 0, & x > a \end{cases}$$

$$F_c(\lambda) = \int_0^a f(x) \cos \lambda x dx$$

$$= \int_0^a \cos x \cos \lambda x dx$$

$$= \frac{1}{2} \int_0^a [\cos(1+\lambda)x + \cos(1-\lambda)x] dx$$

$$= \frac{1}{2} \left[\frac{\sin(1+\lambda)x}{1+\lambda} + \frac{\sin(1-\lambda)x}{1-\lambda} \right]_0^a$$

$$F_c(\lambda) = \frac{1}{2} \left[\frac{\sin(1+\lambda)a}{1+\lambda} + \frac{\sin(1-\lambda)a}{1-\lambda} \right]$$

$$\sin a \sin b = -\frac{1}{2} [\cos(a+b) - \cos(a-b)]$$

$$3. f(x) = \begin{cases} 1-x^2, & |x| \leq 1 \\ 0, & |x| > 1 \end{cases}$$

$$\int_0^{\infty} \left[\frac{x \cos x - \sin x}{x^3} \right] \cos \frac{x}{2} dx$$

Hence evaluate integral

$$f(x) = 1-x^2$$

FCT.

$$F_c(x) = \int_0^{\infty} f(x) \cos xu \, du$$

$$= \int_0^{\infty} (1-x^2) \cos xu \, du$$

$$= \left[(1-x^2) \left(\frac{\sin xu}{x} \right) - (-2x) \left(-\frac{\cos xu}{x^2} \right) + (-2) \left(-\frac{\sin xu}{x^3} \right) \right]_0^{\infty}$$

$$= \left[\frac{-2 \cos x}{x^2} + \frac{2 \sin x}{x^3} \right]$$

$$F_c(x) = 2 \left[\frac{\sin x}{x^3} - \frac{\cos x}{x^2} \right]$$

Now F(1R)

$$f(x) = -\frac{2 \times 2}{\pi} \int_0^{\infty} \left[\frac{x \cos x - \sin x}{x^3} \right] \cos \frac{x}{2} dx$$

$$\int_0^{\infty} \left[\frac{x \cos x - \sin x}{x^3} \right] \cos \frac{x}{2} dx = -f(x) \frac{\pi}{4}$$

$$\text{Let } n = \frac{1}{2}$$

$$\int_0^{\infty} \left(\frac{\lambda \cos \lambda - \sin \lambda}{\lambda^3} \right) \cos \frac{\lambda}{2} d\lambda = -f\left(\frac{1}{2}\right) \frac{\pi}{4}$$

$$f(n) = 1 - n^2$$

$$f\left(\frac{1}{2}\right) = 1 - \frac{1}{4} = \frac{3}{4}$$

$$\int_0^{\infty} \left(\frac{\lambda \cos \lambda - \sin \lambda}{\lambda^3} \right) \cos \frac{\lambda}{2} d\lambda = -\frac{3}{4} \left(\frac{\pi}{4} \right)$$

$$= -\frac{3\pi}{16}, \quad |n| \leq 1$$

$$\text{and } = 0, \quad |n| > 1$$

Type: 3: Problems on inverse Fourier transform

Q. Find inverse transform whose Fourier cosine transform is

$$1) \frac{\sin a\lambda}{\lambda}$$

$$F_c(\lambda) = \frac{\sin a\lambda}{\lambda}$$

To find Inverse

IFCT

$$f(x) = \frac{2}{\pi} \int_0^{\infty} F_c(\lambda) \cos \lambda x d\lambda$$

$$= \frac{2}{\pi} \int_0^{\infty} \frac{\sin a\lambda}{\lambda} \cos \lambda x d\lambda$$

$$= \frac{2}{\pi} \int_0^{\infty} \frac{1}{\lambda} [\sin(a+x)\lambda + \sin(a-x)\lambda] d\lambda$$

$$= \frac{1}{\pi} \left[\int_0^{\infty} \frac{\sin(a+\alpha)\lambda}{\lambda} d\lambda + \int_0^{\infty} \frac{\sin(a-\alpha)\lambda}{\lambda} d\lambda \right]$$

$$= \frac{1}{\pi} \left[\frac{\pi}{2} + \frac{\pi}{2} \right] \quad \begin{array}{l} (a+\alpha) > 0, (a-\alpha) > 0 \\ (a+\alpha) > 0, (a-\alpha) < 0 \end{array}$$

$$= 1$$

$$= \frac{1}{\pi} \left[\frac{\pi}{2} - \frac{\pi}{2} \right]$$

$$= 0$$

2. Solve for integral eq.

$$2) \int f(x) \sin \pi x dx = \begin{cases} 1-x, & 0 \leq x \leq 1 \\ 0, & x > 1 \end{cases}$$

We know that

$$f_s(x) = \int_0^{\infty} f(x) \sin \pi x dx$$

$$f_s(x) = \begin{cases} 1-x, & 0 \leq x \leq 1 \\ 0, & x > 1 \end{cases}$$

Now IFSI

$$f(x) = \frac{2}{\pi} \int_0^{\infty} f_s(\lambda) \sin \pi x d\lambda$$

$$= \frac{2}{\pi} \int_0^1 (1-\lambda) \sin \pi x d\lambda$$

$$= \frac{2}{\pi} \left[(1-\lambda) \left(\frac{-\cos \lambda \pi}{\lambda \pi} \right) - (-1) \left(\frac{-\sin \lambda \pi}{\lambda \pi^2} \right) \right]'$$

$$\frac{2}{\pi} \left[\frac{-\sin \pi}{\pi^2} + \frac{1}{\pi} \right]$$

$$\frac{2}{\pi} \left[\frac{\pi - \sin \pi}{\pi^2} \right]$$

3. Solve the integral eq $\int_0^\infty f(u) \cos \lambda u \, du = \begin{cases} 1-\lambda & 0 \leq \lambda \leq 1 \\ 0 & \lambda > 1 \end{cases}$

Show that $\int_0^\infty \frac{\sin^2 z}{z^2} \, dz = \frac{\pi}{2}$

$$F_c(\lambda) = \int_0^\infty f(u) \cos \lambda u \, du \quad \text{--- (1)}$$

$$F_c(\lambda) = 1 - \lambda, \quad 0 \leq \lambda \leq 1$$

$$= 0, \quad \lambda > 1$$

Now,

IFT

$$f(u) = \frac{2}{\pi} \int_0^\infty F_c(\lambda) \cos \lambda u \, d\lambda$$

$$= \frac{2}{\pi} \int_0^1 (1-\lambda) \cos \lambda u \, d\lambda$$

$$= \frac{2}{\pi} \left[(1-\lambda) \left(\frac{\sin \lambda u}{u} \right) - (-1) \left(\frac{-\cos \lambda u}{u^2} \right) \right]_0^1$$

$$= \frac{2}{\pi} \left[\frac{-\cos u}{u^2} + \frac{1}{u^2} \right]$$

$$f(u) = \frac{2}{\pi} \left[\frac{1 - \cos u}{u^2} \right]$$

$$\text{then } f(u) = \frac{2}{\pi} \left[\frac{1 - \cos u}{u^2} \right]$$

Put $f(u)$ in eq (1)

$$F_c(\lambda) = \int_0^{\infty} \frac{2}{\pi} \left[\frac{1 - \cos u}{u^2} \right] \cos \lambda u \, du$$

$$= \frac{4}{\pi} \int_0^{\infty} \frac{\sin^2 u/2}{u^2} \cos \lambda u \, du$$

Put $\lambda = 0$ because $\cos 0 = 1$

$$F_c(0) = \frac{4}{\pi} \int_0^{\infty} \frac{\sin^2 u/2}{u^2} \, du$$

Put $u/2 = z$

$$\therefore u = 2z$$

$$du = 2dz$$

$$F_c(0) = \frac{4}{\pi} \int_0^{\infty} \frac{\sin^2 z}{4z^2} 2dz$$

$$F_c(0) = \frac{2}{\pi} \int_0^{\infty} \frac{\sin^2 z}{z^2} dz$$

$$\frac{\pi}{2} F_c(0) = \int_0^{\infty} \frac{\sin^2 z}{z^2} dz$$

$$\int_0^{\infty} \frac{\sin^2 z}{z^2} dz = \frac{\pi}{2} F_c(0)$$

$$F_c(\lambda) = 1 - \lambda, \quad 0 \leq \lambda < 1$$

$$F_c(0) = 1 - 0$$

$$= 1$$

$$0 \leq \lambda < 1$$

$$\therefore F_c(0) = 0, \quad \lambda \geq 1$$

$$\therefore \int_0^{\infty} \frac{\sin^2 z}{z^2} dz = \frac{\pi}{2}, \quad 0 < \lambda < 1$$

$$\int_0^{\infty} \frac{\sin^2 z}{z^2} dz = 0, \quad \lambda \geq 1$$

Q. Solve the foll. integral

$$\int_0^{\infty} f(u) \sin \lambda u \, d\lambda = \begin{cases} 1, & 0 < \lambda < 1 \\ 2, & 1 < \lambda < 2 \\ 0, & \lambda > 2 \end{cases}$$

~~$$F_s(\lambda) = \int_0^{\infty} f(u) \sin \lambda u \, du$$~~

$$F_s(\lambda) = \int_0^{\infty} f(u) \sin \lambda u \, du \quad - (1)$$

Now IFSI

$$f(u) = \frac{2}{\pi} \int_0^{\infty} F_s(\lambda) \sin \lambda u \, d\lambda$$

$$f(u) = \frac{2}{\pi} \int_0^1 (1) \sin \lambda u \, d\lambda + \frac{2}{\pi} \int_1^2 (2) \sin \lambda u \, d\lambda + \int_2^{\infty} 0$$

$$\frac{2}{\pi} \left[\left(-\frac{\cos \lambda u}{u} \right)_0^1 + \left(-\frac{2 \cos \lambda u}{u} \right)_1^2 \right]$$

$$\frac{2}{\pi} \left[-\frac{\cos u}{u} + \frac{1}{u} - \frac{2 \cos 2u}{u} + \frac{2 \cos u}{u} \right]$$

$$f(u) = \frac{2}{\pi} \left[\frac{\cos u}{u} - \frac{2 \cos 2u}{u} + \frac{1}{u} \right]$$

Q. Find inverse transform if ~~$e^{-\lambda}$~~

$$F_c(\lambda) = e^{-\lambda}, \quad \lambda > 0$$

$$F_c(\lambda) = \int_0^{\infty} f(x) \cos \lambda x \, dx$$

Now IFT ∞

$$f(x) = \frac{2}{\pi} \int_0^{\infty} F_c(\lambda) \cos \lambda x \, d\lambda$$

$$f(x) = \frac{2}{\pi} \int_0^{\infty} e^{-\lambda} \cos \lambda x \, d\lambda$$

$$a=1, b=x$$

$$= \frac{2}{\pi} \left[\frac{1}{1+x^2} \right]$$